\documentclass{article}
\usepackage{amsmath,amsthm}
\usepackage{cancel}
\usepackage{indentfirst}
\usepackage{commath}
\begin{document}

% TODO: Pull this into a common file
% From Wikipedia, not sure where to define this yet...
\def\ci{\perp\!\!\!\perp}
\def\defeq{\buildrel\triangle\over =}
\def\E{\mathrm{E}}
\def\Var{\mathrm{Var}}
\def\Cov{\mathrm{Cov}}


\section{MLE for the Bernoulli/ binomial model}

\begin{gather}
X_i \sim Ber(\theta) \\
p(D|\theta) = \theta^{N_1}(1 - \theta)^{N_0}
\end{gather}

\begin{align*}
  \ln \left(  p(D|\theta) \right) &= \ln \left( \theta^{N_1}(1 -
                                    \theta)^{N_0} \right) \\
                                  &= \ln \left( \theta^{N-1} \right) + \ln \left( 1 - \theta
                                    \right)^{N_0} \\
                                  &= N_1 \ln \theta + N_0 \ln (1 - \theta) \\
  \od{}{\theta} \ln p(D|\theta) &= \frac{N_1}{\theta} - \frac{N_0}{1 -
                                  \theta}
\end{align*}

The log-likelihood will take a maximum when the derivative equals 0.

\begin{align*}
  0 &= \frac{N_1}{\theta} - \frac{N - N_1}{1 - \theta} \\
  0 &= N_1(1 - \theta) - \theta(N-N_1) \\
  0 &= N_1 - \theta N_1 - \theta N + \theta N_1 \\
  0 &= N_1 - \theta(N_1 + N - N_1) \\
  0 &= N_1 - \theta N \\
  \hat{\theta} &= \frac{N_1}{N}
\end{align*}
\section{Marginal likelihood for Beta-Bernoulli model}
\begin{equation}\label{chain-rule-prob}
  p(X_{1:N}) = p(x_1)p(x_2|x_1)p(x_3|x_{1:2}) ... p(x_N|x_{N-1})
\end{equation}

\begin{equation}\label{bb-post-pred}
    p(X=k|D_{1:N}) = \frac{N_k + \alpha_k}{\sum_i N_i + \alpha_i}
\end{equation}

\begin{equation}\label{gamma-def}
  (\alpha - 1)! = \Gamma(\alpha)
\end{equation}

Given $D = H,T,T,H,H \defeq 1,0,0,1,1$

\begin{gather*}
  p(X=1|\alpha) = \frac{\alpha_1}{\alpha} \\
  p(X=0|\alpha, D_1) = \frac{\alpha_0}{\alpha + 1} \\
  p(X=0|\alpha, D_{1:2}) = \frac{\alpha_0 + 1}{\alpha + 2} \\
  p(X=1|\alpha, D_{1:3}) = \frac{\alpha_0 + 1}{\alpha + 3} \\
  p(X=1|\alpha, D_{1:4}) = \frac{\alpha_0 + 2}{\alpha + 4} \\
\end{gather*}

\begin{align*}
  p(D) &= p(D_{1:5}) \\
       &= p(D_1) \cdot p(D_2|D_1) \cdot p(D_3|D_{1:2}) \cdot
         p(D_4|D_{1:3}) \cdot p(D_5|D_{1:4}) \qquad \text{by ($\ref{chain-rule-prob}$)} \\
       &= \frac{\alpha_1}{\alpha} \cdot
         \frac{\alpha_0}{\alpha + 1} \cdot \frac{\alpha_0 + 1}{\alpha + 2}
         \cdot \frac{\alpha_1 + 1}{\alpha + 3} \cdot \frac{\alpha_1 +
         2}{\alpha + 4} \qquad \text{by ($\ref{bb-post-pred}$)} \\
       &= \frac{\left[ \alpha_1 (\alpha_1 + 1) (\alpha_1 + 2) \right] \left[
         \alpha_0 (\alpha_0 + 1) \right]}
         {\alpha (\alpha + 1) (\alpha + 2) (\alpha + 3) (\alpha + 4) }
  \\
       &= \frac{\left[ (\alpha_1) ... (\alpha_1 + N_1 - 1) \right] \left[
         (\alpha_0) ... (\alpha_0 + N_0 - 1) \right]}
         {(\alpha) ... (\alpha + N - 1)} \\
       &= \frac{(\alpha_1 + N_1 - 1)!}{(\alpha_1 - 1)!} \cdot
         \frac{(\alpha_0 + N_0 - 1)!}{(\alpha_0 - 1)!} \cdot
         \frac{(\alpha - 1)!}{(\alpha + N - 1)!} \\
       &= \frac{\Gamma(\alpha_1 + N_1)}{\Gamma(\alpha_1)} \cdot \frac{\Gamma(\alpha_0
         + N_0)}{\Gamma(\alpha_0)} \cdot
         \frac{\Gamma(\alpha)}{\Gamma(\alpha + N)} \\
       &= \frac{\Gamma(\alpha_1 + N_1) \; \Gamma(\alpha_0 +
         N_0)}{\Gamma(\alpha_1) \Gamma(\alpha_0)}
         \frac{\Gamma(\alpha_0 + \alpha_1)}{\Gamma(\alpha_0 + \alpha_1 +
         N)}
\end{align*}

\section{Posterior predictive for a Beta-Binomial model}

\begin{align*}
  p(x|n,D) &= Bb(x|\alpha_0', \alpha_1', n) \\
  &= \frac{B(x + \alpha_1', n-x+\alpha_0')}{B(\alpha_1',\alpha_0')} {n
    \choose x}
\end{align*}

Given $n = 1$

\begin{align*}
  Bb(1|\alpha_0,\alpha_1,1) &= \frac{B(1 + \alpha_1,
                              \alpha_0)}{B(\alpha_1, \alpha_0)} {1
                              \choose 1} \\
                            &= \frac{\Gamma(1 + \alpha_1)
                              \Gamma(\alpha_0)}{\Gamma(\alpha_0 +
                              \alpha_1 + 1)} \cdot
                              \frac{\Gamma(\alpha_0 +
                              \alpha_1)}{\Gamma(\alpha_0)\Gamma(\alpha_1)}
  \\
                            &= \frac{\alpha_1 \Gamma(\alpha_1)
                              \Gamma(\alpha_0)}{(\alpha_0 + \alpha_1)
                              \Gamma(\alpha_0 + \alpha_1)} \cdot
                              \frac{\Gamma(\alpha_0 +
                              \alpha_1)}{\Gamma(\alpha_0)\Gamma(\alpha_1)}
  \\
                            &= \frac{\alpha_1}{\alpha_0 + \alpha_1} \\
                            &= \frac{\alpha_1}{\alpha}
\end{align*}



\end{document}
